Rewrite expression compiler, complete proof

PyLevelLang/src/PyLevelLang/Compile.v
@@ -1,22 +1,33 @@
 Require Import PyLevelLang.Language.
+Require Import PyLevelLang.Interpret.
+Require Import PyLevelLang.Elaborate.
 Require bedrock2.Syntax.
+Require Import bedrock2.Semantics.
 Require Import coqutil.Datatypes.Result.
 Import ResultMonadNotations.
+Require Import coqutil.Map.Interface coqutil.Map.SortedListString.
+Require Import coqutil.Byte coqutil.Word.Interface coqutil.Word.Bitwidth coqutil.Word.Properties.
+
+Require Import coqutil.Tactics.fwd.
+
+Context {width: Z} {BW: Bitwidth width} {word: word.word width} {mem: map.map word byte}.
+Context {word_ok: word.ok word} {mem_ok: map.ok mem}.
 
 Definition compile_atom {t : type} (a : atom t) : result Syntax.expr :=
   match a with
-  | AInt n => Success (Syntax.expr.literal n)
+  | AWord z => Success (Syntax.expr.literal z)
   | ABool b => Success (Syntax.expr.literal (Z.b2z b))
-  | AString _ | ANil _ | AEmpty => error:("unimplemented")
+  | AInt _ | AString _ | ANil _ | AEmpty => error:("unimplemented")
   end.
 
 Definition compile_unop {t1 t2 : type} (o : unop t1 t2) :
   result (Syntax.expr -> Syntax.expr) :=
   match o with
-  | ONeg =>
+  | OWNeg =>
       Success (Syntax.expr.op Syntax.bopname.sub (Syntax.expr.literal 0))
   | ONot =>
-      Success (Syntax.expr.op Syntax.bopname.sub (Syntax.expr.literal 0))
+      Success (Syntax.expr.op Syntax.bopname.sub (Syntax.expr.literal 1))
+  | ONeg
   | OLength _
   | OLengthString
   | OFst _ _ _
@@ -27,18 +38,16 @@ Definition compile_unop {t1 t2 : type} (o : unop t1 t2) :
 Definition compile_binop {t1 t2 t3 : type} (o : binop t1 t2 t3) :
   result (Syntax.expr -> Syntax.expr -> Syntax.expr) :=
   match o with
-  | OPlus =>
+  | OWPlus =>
       Success (Syntax.expr.op Syntax.bopname.add)
-  | OMinus =>
+  | OWMinus =>
       Success (Syntax.expr.op Syntax.bopname.sub)
-  | OTimes =>
+  | OWTimes =>
       Success (Syntax.expr.op Syntax.bopname.mul)
-  | ODiv =>
+  | OWDivU =>
       Success (Syntax.expr.op Syntax.bopname.divu)
-      (* FIXME *)
-  | OMod =>
+  | OWModU =>
       Success (Syntax.expr.op Syntax.bopname.remu)
-      (* FIXME *)
   | OAnd =>
       Success (Syntax.expr.op Syntax.bopname.and)
   | OOr =>
@@ -46,11 +55,20 @@ Definition compile_binop {t1 t2 t3 : type} (o : binop t1 t2 t3) :
   | OConcat _
   | OConcatString =>
       error:("unimplemented")
-  | OLess =>
+  | OWLessU =>
       Success (Syntax.expr.op Syntax.bopname.ltu)
-      (* FIXME *)
+  | OWLessS =>
+      Success (Syntax.expr.op Syntax.bopname.lts)
   | OEq _ H =>
       Success (Syntax.expr.op Syntax.bopname.eq)
+  | OPlus
+  | OMinus
+  | OTimes
+  | OWDivS
+  | ODiv
+  | OWModS
+  | OMod
+  | OLess
   | ORepeat _
   | OPair _ _ _
   | OCons _
@@ -73,8 +91,167 @@ Fixpoint compile_expr {t : type} (e : expr t) : result Syntax.expr :=
   | _ => error:("unimplemented")
   end.
 
-Compute (compile_expr (EAtom (AInt 4))).
+Section WithMap.
+  Context {tenv : map.map string (type * bool)} {tenv_ok : map.ok tenv}.
+  Context {locals: map.map string {t & interp_type (word := word) t}} {locals_ok: map.ok locals}.
+  (* Context {width: Z} {BW: Bitwidth width} {word: word.word width} {mem: map.map word byte}. *)
+  (* Context {word_ok: word.ok word} {mem_ok: map.ok mem}. *)
+  Context {locals': map.map string word} {locals'_ok: map.ok locals}.
+
+  Inductive value_relation : forall {t : type}, interp_type t -> word -> Prop :=
+    | RWord (w : word) : value_relation (t := TWord) w w
+    | RBool (b : bool) : value_relation (t := TBool) b (word.of_Z (Z.b2z b)).
+
+  Lemma RBool' (b : bool) (w : word) : w = word.of_Z (Z.b2z b) ->
+    value_relation (t := TBool) b w.
+  Proof.
+    intros [= ->].
+    apply RBool.
+  Qed.
+
+  (* Prove lemmas for opposite directions *)
+
+  (* Definition compile_value {t : type} (v : interp_type t) : result word := *)
+  (*   match t as t' return interp_type t' -> _ with *)
+  (*   | TInt => fun v => Success (word.of_Z v) *)
+  (*   | TBool => fun v => Success (word.of_Z (Z.b2z v)) *)
+  (*   | _ => fun _ => error:("unimplemented") *)
+  (*   end v. *)
+
+  Lemma interp_type_eq : forall {t : type} (e : expr t) (w : interp_type t),
+    (existT interp_type t w =
+    existT interp_type t (interp_expr (locals := locals) map.empty e)) ->
+    (interp_expr map.empty e) = w.
+  Proof.
+    intros.
+    inversion_sigma.
+    rewrite <- Eqdep_dec.eq_rect_eq_dec in H0.
+    * easy.
+    * exact type_eq_dec.
+  Qed.
+
+  Lemma compile_correct : forall {t} (e : expr t) (e' : Syntax.expr),
+    wf map.empty e ->
+    compile_expr e = Success e' -> exists w,
+    eval_expr_old map.empty map.empty e' = Some w /\
+    value_relation (interp_expr map.empty e) w.
+  Proof.
+    intros t. induction e; intros e' He He'; try easy.
+    - (* EAtom a *)
+      destruct a; try easy.
+      + (* AInt n *)
+        injection He' as [= <-].
+        simpl.
+        exists (word.of_Z (word.wrap n)).
+        split; rewrite <- word.unsigned_of_Z, word.of_Z_unsigned; try easy.
+        apply RWord.
+      + (* ABool b *)
+        injection He' as [= <-].
+        simpl.
+        exists (word.of_Z (Z.b2z b)).
+        split; try easy.
+        apply RBool.
+    - (* EUnop o e *)
+      destruct o; try easy.
+      all:
+        simpl in He';
+        simpl;
+        fwd;
+        inversion He;
+        injection H4 as [= ->];
+        specialize IHe with (1 := H2) (2 := eq_refl);
+        fwd;
+        eexists.
+      + (* OWNeg *)
+        split.
+        * simpl. fwd.
+          now rewrite Properties.word.sub_0_l.
+        * inversion IHep1. rewrite H6 in H5.
+          rewrite (interp_type_eq _ _ H5).
+          apply RWord.
+      + (* ONot *)
+        split.
+        * simpl. now fwd.
+        * inversion IHep1.
+          rewrite (interp_type_eq _ _ H5).
+          rewrite <- Properties.word.ring_morph_sub.
+          destruct b; apply RBool.
+    - (* EBinop o e1 e2 *)
+      destruct o; try easy.
+      all:
+        simpl in He';
+        simpl;
+        fwd;
+        inversion He;
+        injection H5 as [= ->];
+        injection H6 as [= ->];
+        injection H5 as [= ->];
+        specialize IHe1 with (1 := H3) (2 := eq_refl);
+        specialize IHe2 with (1 := H7) (2 := eq_refl);
+        fwd;
+        eexists.
+      1, 2, 3, 4, 5:
+        (* OWPlus, OWMinus, OWTimes, OWDivU, OWModU *)
+        split;
+        [ simpl; now fwd
+        | inversion IHe1p1; inversion IHe2p1;
+          rewrite H6 in H5; rewrite H9 in H8;
+          rewrite (interp_type_eq _ _ H5);
+          rewrite (interp_type_eq _ _ H8);
+          apply RWord ].
+      1, 2:
+        (* OAnd, OOr *)
+        split;
+        [ simpl; now fwd
+        | inversion IHe1p1; inversion IHe2p1;
+          rewrite (interp_type_eq _ _ H5);
+          rewrite (interp_type_eq _ _ H8);
+          destruct b, b0;
+            simpl;
+            apply RBool';
+            apply word.unsigned_inj;
+            simpl Z.b2z;
+            try rewrite word.unsigned_and_nowrap;
+            try rewrite word.unsigned_or_nowrap;
+            now try rewrite word.unsigned_of_Z_0;
+            try rewrite word.unsigned_of_Z_1 ].
+      1, 2:
+        (* OWLessU, OWLessS *)
+        split;
+        [ simpl; now fwd
+        | inversion IHe1p1; inversion IHe2p1;
+          rewrite (interp_type_eq _ _ H5);
+          rewrite (interp_type_eq _ _ H8);
+          rewrite H6, H9;
+          (destruct (word.ltu w0 w); apply RBool)
+          || (destruct (word.lts w0 w); apply RBool) ].
+      (* OEq *)
+      + split.
+        * simpl; now fwd.
+        * destruct t; try easy; unfold eqb_values.
+          -- (* TWord *)
+             inversion IHe1p1. inversion IHe2p1.
+             rewrite (interp_type_eq _ _ H5).
+             rewrite (interp_type_eq _ _ H8).
+             rewrite H6, H9.
+             destruct (word.eqb w0 w); apply RBool.
+          -- (* TBool *)
+             inversion IHe1p1. inversion IHe2p1.
+             rewrite (interp_type_eq _ _ H5).
+             rewrite (interp_type_eq _ _ H8).
+             rewrite H6, H9.
+             destruct b, b0.
+             all:
+               destruct (word.eqb w0 w) eqn:Heq; try now apply RBool'.
+             1, 4: rewrite <- H6, <- H9 in Heq; now apply word.eqb_false in Heq.
+             all:
+               rewrite <- H6, <- H9 in Heq; apply word.eqb_true in Heq;
+               simpl in Heq; (rewrite Heq || rewrite <- Heq); apply RBool.
+  Qed.
+End WithMap.
+
+Compute (compile_expr (EAtom (AWord 4))).
 Compute (compile_expr (EAtom (ABool true))).
 Compute (compile_expr (EAtom (ABool false))).
 Compute (compile_expr (EBinop OOr (EAtom (ABool true)) (EAtom (ABool false)))).
-Compute (compile_expr (EBinop OPlus (EAtom (AInt 1)) (EAtom (AInt 1)))).
+Compute (compile_expr (EBinop OWPlus (EAtom (AWord 1)) (EAtom (AWord 1)))).
